common/LinkerProp.v
@@ -10,12 +10,11 @@ Set Implicit Arguments.
 
 Section LINKER_PROP.
 
-Variable (fundefT F EF V:Type).
-Variable (fundef_dec: fundef_decT fundefT F EF).
-Variable (EF_dec: forall (v1 v2:EF), {v1 = v2} + {v1 <> v2}).
+Variable (fundefT F V:Type).
+Variable (fundef_dec: fundef_decT fundefT F).
 Variable (V_dec: forall (v1 v2:V), {v1 = v2} + {v1 <> v2}).
 
-Lemma gflink_globdefs defs1 defs2 (Hlink: link_globdefs fundef_dec EF_dec V_dec defs1 defs2 = None):
+Lemma gflink_globdefs defs1 defs2 (Hlink: link_globdefs fundef_dec V_dec defs1 defs2 = None):
   exists var def1 def2,
     PTree.get var defs1 = Some def1 /\
     PTree.get var defs2 = Some def2 /\
@@ -31,12 +30,12 @@ Proof.
   destruct Hlinkable as [i [x [Hx1 Hx2]]].
   destruct x; inv Hx2. rewrite PTree.gcombine in Hx1; auto.
   destruct (defs1 ! i) eqn:Hi1, (defs2 ! i) eqn:Hi2; inv Hx1.
-  destruct (globdef_linkable_dec fundef_dec EF_dec V_dec g g0); inv H0.
-  destruct (globdef_linkable_dec fundef_dec EF_dec V_dec g0 g); inv H1.
+  destruct (globdef_linkable_dec fundef_dec V_dec g g0); inv H0.
+  destruct (globdef_linkable_dec fundef_dec V_dec g0 g); inv H1.
   repeat eexists; eauto.
 Qed.
 
-Lemma gtlink_globdefs defs1 defs2 defs (Hlink: link_globdefs fundef_dec EF_dec V_dec defs1 defs2 = Some defs):
+Lemma gtlink_globdefs defs1 defs2 defs (Hlink: link_globdefs fundef_dec V_dec defs1 defs2 = Some defs):
   forall var,
     match PTree.get var defs1, PTree.get var defs2, PTree.get var defs with
       | Some g1, Some g2, Some g =>
@@ -55,16 +54,16 @@ Proof.
   end.
   rewrite PTree.goption_map, PTree.gcombine; auto.
   destruct (defs1 ! i) eqn:Hi1, (defs2 ! i) eqn:Hi2; auto.
-  destruct (globdef_linkable_dec fundef_dec EF_dec V_dec g g0).
+  destruct (globdef_linkable_dec fundef_dec V_dec g g0).
   { left. split; auto. }
-  destruct (globdef_linkable_dec fundef_dec EF_dec V_dec g0 g).
+  destruct (globdef_linkable_dec fundef_dec V_dec g0 g).
   { right. split; auto. }
   eapply PTree_Properties.for_all_correct in Hlinkable; eauto.
   { instantiate (1 := None) in Hlinkable. inv Hlinkable. }
   instantiate (1 := i). rewrite PTree.gcombine; auto.
   rewrite Hi1, Hi2.
-  destruct (globdef_linkable_dec fundef_dec EF_dec V_dec g g0); try (contradict n; auto; fail).
-  destruct (globdef_linkable_dec fundef_dec EF_dec V_dec g0 g); try (contradict n0; auto; fail).
+  destruct (globdef_linkable_dec fundef_dec V_dec g g0); try (contradict n; auto; fail).
+  destruct (globdef_linkable_dec fundef_dec V_dec g0 g); try (contradict n0; auto; fail).
   auto.
 Qed.
 
